TStream_DS.thy
@@ -11,68 +11,7 @@ imports TStream OptionCpo (* "~~/src/HOL/HOLCF/Library/Option_Cpo" *)
 
 begin  
 default_sort countable
-
-(* ----------------------------------------------------------------------- *)
-subsection {* tsRemDups *}
-(* ----------------------------------------------------------------------- *)   
-
-fixrec tsRemDups_h :: "'a tstream \<rightarrow> 'a discr option \<rightarrow> 'a tstream" where
-  (* ignore ticks *)
-"tsRemDups_h\<cdot>(tsLscons\<cdot>(up\<cdot>DiscrTick)\<cdot>ts)\<cdot>option = delayFun\<cdot>(tsRemDups_h\<cdot>ts\<cdot>option)"  | 
-
-  (* handle first message *)
-"ts\<noteq>\<bottom> \<Longrightarrow> tsRemDups_h\<cdot>(tsLscons\<cdot>(up\<cdot>(uMsg\<cdot>t))\<cdot>ts)\<cdot>None = tsMLscons\<cdot>(up\<cdot>t)\<cdot>(tsRemDups_h\<cdot>ts\<cdot>(Some t))" | 
-
-  (* handle duplicate message *)
-"ts\<noteq>\<bottom> \<Longrightarrow> tsRemDups_h\<cdot>(tsLscons\<cdot>(up\<cdot>(uMsg\<cdot>t))\<cdot>ts)\<cdot>(Some a) = 
-  (if t=a then (tsRemDups_h\<cdot>ts\<cdot>(Some t)) else tsMLscons\<cdot>(up\<cdot>t)\<cdot>(tsRemDups_h\<cdot>ts\<cdot>(Some t)))"   
-
-declare tsRemDups_h.simps [simp del]
-
-definition tsRemDups :: "'a tstream \<rightarrow> 'a tstream" where
-"tsRemDups \<equiv> \<Lambda> ts. tsRemDups_h\<cdot>ts\<cdot>None"
-
-lemma tsRemDups_insert: "tsRemDups\<cdot>ts = tsRemDups_h\<cdot>ts\<cdot>None"
-by (simp add: tsRemDups_def)
-
-lemma tsremdups_h_strict [simp]: 
-"tsRemDups_h\<cdot>\<bottom>\<cdot>a = \<bottom>"
-by (fixrec_simp)
-
-lemma tsremdups_h_tslscons_fst [simp]: 
-  "ts\<noteq>\<bottom> \<Longrightarrow> tsRemDups_h\<cdot>(tsLscons\<cdot>(up\<cdot>(uMsg\<cdot>t))\<cdot>ts)\<cdot>None = tsMLscons\<cdot>(up\<cdot>t)\<cdot>(tsRemDups_h\<cdot>ts\<cdot>(Some t))"
-by (fixrec_simp)
-
-lemma tsremdups_h_tslscons_dup [simp]: 
-  "ts\<noteq>\<bottom> \<Longrightarrow> tsRemDups_h\<cdot>(tsLscons\<cdot>(up\<cdot>(uMsg\<cdot>t))\<cdot>ts)\<cdot>(Some a) 
-          = (if t=a then (tsRemDups_h\<cdot>ts\<cdot>(Some t)) else tsMLscons\<cdot>(up\<cdot>t)\<cdot>(tsRemDups_h\<cdot>ts\<cdot>(Some t)))"
-by (fixrec_simp)
-
-lemma tsremdups_h_tslscons_tick [simp]: 
-  "tsRemDups_h\<cdot>(tsLscons\<cdot>(up\<cdot>DiscrTick)\<cdot>ts)\<cdot>option = delayFun\<cdot>(tsRemDups_h\<cdot>ts\<cdot>option)"
-by (fixrec_simp)
-
-(* handle first message *)
-lemma tsremdups_h_mlscons:
-"ts\<noteq>\<bottom> \<Longrightarrow> tsRemDups_h\<cdot>(tsMLscons\<cdot>(up\<cdot>t)\<cdot>ts)\<cdot>None = tsMLscons\<cdot>(up\<cdot>t)\<cdot>(tsRemDups_h\<cdot>ts\<cdot>(Some t))"
-by (simp add: tsmlscons_lscons)
-
-(* handle duplicate message *)
-lemma tsremdups_h_mlscons_dup: 
-  "ts\<noteq>\<bottom> \<Longrightarrow> tsRemDups_h\<cdot>(tsMLscons\<cdot>(up\<cdot>t)\<cdot>ts)\<cdot>(Some t) = tsRemDups_h\<cdot>ts\<cdot>(Some t)"
-by (simp add: tsmlscons_lscons)
-
-(* handle message *)
-lemma tsremdups_h_mlscons_ndup:
-  "ts\<noteq>\<bottom> \<Longrightarrow> t\<noteq>a \<Longrightarrow> tsRemDups_h\<cdot>(tsMLscons\<cdot>(up\<cdot>t)\<cdot>ts)\<cdot>(Some a) 
-                               = tsMLscons\<cdot>(up\<cdot>t)\<cdot>(tsRemDups_h\<cdot>ts\<cdot>(Some t))"
-by (simp add: tsmlscons_lscons)
-
-lemma tsremdups_h_delayfun: "tsRemDups_h\<cdot>(delayFun\<cdot>ts)\<cdot>a = delayFun\<cdot>(tsRemDups_h\<cdot>ts\<cdot>a)"
-by (simp add: delayfun_tslscons)
-
-
-  
+ 
 lift_definition tsExampIn :: "nat tstream" is "<[Msg 1, Msg 2, \<surd>, Msg 2, \<surd>]>"
 by (subst ts_well_def, auto)
 
